
\subsection{11.1 $\bigstar\bigstar$}
For the first, 
\begin{align*}\mathbf{i}\mathbf{j}\mathbf{k}=-1\implies\mathbf{i}(\mathbf{i}\mathbf{j}\mathbf{k})=-\mathbf{i}\implies(\mathbf{i}\mathbf{i})\mathbf{j}\mathbf{k}=-\mathbf{i}&\implies-\mathbf{j}(\mathbf{j}\mathbf{k})=-\mathbf{j}\mathbf{i}\\
&\implies \mathbf{k}=-\mathbf{j}\mathbf{i}
\end{align*}
But also $\mathbf{i}\mathbf{j}\mathbf{k}=-1\implies(\mathbf{i}\mathbf{j}\mathbf{k})\mathbf{k}=-\mathbf{k}\implies\mathbf{i}\mathbf{j}=\mathbf{k}$. Hence $\mathbf{i}\mathbf{j}=\mathbf{k}=-\mathbf{j}\mathbf{i}$, as we wanted. The other two are done using the same technique.



