% --------------------------------------
% Chapter 9 Solutions
% --------------------------------------

\subsection{9.1 $\bigstar$}
For a given frequency $n\omega$, we have two contributing exponentials 
\begin{align*}
\alpha_{-n} e^{-in \omega}+\alpha_n e^{in \omega}&=\alpha_{-n}[\cos (-n\omega)+i\sin (-n\omega)]+\alpha_n[\cos (n\omega)+i\sin (n\omega)]\\
&=(\alpha_{-n}+\alpha_n)\cos (n\omega)+i(\alpha_{-n}-\alpha_n)\sin (n\omega)\\
&=a_n\cos (n\omega)+b_n\sin (n\omega)
\end{align*} 
where we made use of $\cos(-x)=\cos x$ and $\sin (-x)=-\sin x$.


\subsection{9.2 $\bigstar \bigstar$}
We learnt on pg.126 that only the $z^{-1}$ term contributes to the integral \footnote{ie. $\oint z^{-1}\,\rm{d}z=2\pi i$ and that $\oint z^{n}\,\rm{d}z=0$ for all $n\neq -1$.} and hence, taking a contour\footnote{obviously the contour will be contained within the unit circle, as this is the region of analyticity of $F(z)$.} about $z=0$, we get
\begin{align*}
\oint z^{-n-1} F(z)\, \text{d}z&=\oint \frac{1}{z^{n+1}} \left (\ldots +\alpha_{n-1}z^{n-1}+\alpha_{n}z^{n}+\alpha_{n+1}z^{n+1}+\ldots \right )\, \text{d}z\\
&= \ldots +\alpha_{n-1}\oint z^{-2} \, \text{d}z+\alpha_{n} \oint z^{-1}\, \text{d}z+\alpha_{n+1}\oint \, \text{d}z+\ldots \\
&=\ldots 0+2\pi i\cdot \alpha_n +0+\ldots\\
&=2\pi i \alpha_n
\end{align*}
The result follows from this.
